TA_Network/TP_NTA_Reduction_Base.thy
@@ -1,5 +1,0 @@
-theory TP_NTA_Reduction_Base
-  imports Main
-begin 
-
-edn
