Temporal_Planning_Base/Error_List_Monad_Add.thy
@@ -1,5 +1,5 @@
 theory Error_List_Monad_Add
-  imports "TA_Library.Error_List_Monad"
+  imports "TA_Impl.Error_List_Monad"
           Temporal_Planning_Base.Base
 begin
 
